\input{./src/main.sty}
% Additional SI unit for Fahrenheit
\DeclareSIUnit\fahrenheit{\degree F}

\begin{document}

% Include title page
\input{./src/titlepage.tex}

\pagebreak

\section*{Problem 6.2.1}% {{{

Solve the problem above of an electron in a potential well with 3
units of field using the first two energy eigenfunctions of the well
without field as the finite basis subset. Give the energies (in the
dimensionless units) and explicit formulae for the normalized
eigenfunctions for the first two levels calculated by this method. Do
the algebra of this problem by hand, i.e., do not use mathematical
software to evaluate matrix elements or to solve for the eigenvalues
and eigenfunctions.

[Note: $\int_0^1(\xi-1/2)\sin(\pi\xi)\sin(2\pi\xi)d\xi=-(8/9\pi^2)$]

\begin{figure}[h]
  \centering
  \includegraphics[width=0.35\textwidth]{./assets/fig_6_2_1.png}
\end{figure}

\boxedanswer{

  The original Hamiltonian is:

  \begin{align*}
    V(z) &= e\mathrm{E}(z - L_z/2) \\
    \hat H &= -\frac{\hbar^2}{2m}\frac{d^2}{dz^2} + e\mathrm{E}(z - L_z/2) \\
  \end{align*}

  Some definitions:

  \begin{align*}
    E_1^\infty &=
    \left(\frac{\hbar^2}{2}\right)\left(\frac{\pi}{L_z}\right)^2 \\ \\
    \eta_n &= \frac{E_n}{E_1^\infty} \text{\qquad(Dimensionless
    eigenenergy of the $n$\textsuperscript{th} eigenstate.)}\\
    \mathrm{E}_o &= \frac{E_o}{eL_z} \\
    \mathrm{f} &= \mathrm{\frac{E}{E_o}} \text{\qquad Dimensionless field} \\
    \xi &= \frac{z}{L_z} \text{\qquad Dimensionless length}
  \end{align*}

  $E_n$ is the well eigenenergy, $E_1^\infty$ is the confinement energy of
  the first state of the infinite well.

  The Hamiltonian becomes:

  \begin{equation*}
    \hat H = -\frac{1}{\pi^2}\frac{d^2}{d\xi^2} + f(\xi - 1/2)
  \end{equation*}

  The unperturbed Schr\"odinger equation:

  \begin{equation*}
    \hat H_o \psi_n = \varepsilon_n\psi_n
  \end{equation*}

}

\pagebreak

\boxedanswer{

  And the general solution:

  \begin{equation*}
    \psi_n(\xi) = \sqrt{2}\sin(n\pi\xi)
  \end{equation*}

  We can construct the Hamiltonian as a matrix:

  \begin{align*}
    H_{ij} &= -\frac{1}{\pi^2} \int_0^1 \psi_i^*(\xi)
    \frac{d^2}{d\xi^2} \psi_j(\xi) d\xi + f\int_0^1 \psi_i^*(\xi)(\xi
    - 1/2)\phi_j(\xi) d\xi
  \end{align*}

  By taking the basis as the first three eignfunctions, we range $i$ and $j$
  from 1 to 2.

  \begin{align*}
    H_{1,1} &= -\frac{1}{\pi^2} \int_0^1 \psi_i^*(\xi) \frac{d^2}{d\xi^2}
    \psi_j(\xi) d\xi + f\int_0^1 \psi_i^*(\xi)(\xi - 1/2)\psi_j(\xi) d\xi \\
    &
    \begin{aligned}
      \psi_1(\xi) &= \psi_1^*(\xi) = \sqrt{2}\sin(\pi\xi) \\
      \frac{d^2}{d\xi^2} \psi_j(\xi) &= -\sqrt{2}\pi^2\sin(\pi\xi) \\
    \end{aligned} \\
    H_{1,1} &= -\frac{1}{\pi^2} \int_0^1 \left(\sqrt{2}\sin(\pi\xi)\right)
    \left(-\sqrt{2}\pi^2\sin(\pi\xi)\right) d\xi +
    f\int_0^1 (\xi - 1/2)\left(\sqrt{2}\sin(\pi\xi)\right)^2 d\xi \\
    H_{1,1} &= 2\pi^2\frac{1}{\pi^2} \int_0^1 \sin^2(\pi\xi)
    d\xi + 2f\int_0^1 (\xi - 1/2)\sin^2(\pi\xi)
    d\xi \\
    &
    \begin{aligned}
      2f\int_0^1 \overbrace{(\xi - 1/2)}^{\text{odd}}\overbrace{\sin^2(\pi\xi)^2
      }^{\text{even}}d\xi &= 0 \\
      2\int_0^1 \sin^2(\pi\xi) d\xi &=
      2\int_0^1\frac{1}{2}\left[1 - \cos(2\pi\xi) \right]d\xi \\
      2\int_0^1 \sin^2(\pi\xi) d\xi &=
      \left[\xi - \frac{1}{2\pi}\sin(2\pi\xi)\right]_0^1 \\
      2\int_0^1 \sin^2(\pi\xi) d\xi &= 1 \\
    \end{aligned} \\ H_{2,2} &= -\frac{1}{\pi^2} \int_0^1
    \psi_2^*(\xi) \frac{d^2}{d\xi^2}
    \psi_2(\xi) d\xi + f\int_0^1 \psi_2^*(\xi)(\xi - 1/2)\psi_2(\xi) d\xi \\
    &
    \begin{aligned}
      \frac{d^2}{d\xi^2} \psi_2(\xi) &= -4\sqrt{2}\pi^2\sin(2\pi\xi) \\
    \end{aligned} \\
    H_{2,2} &= 8\int_0^1\sin^2(2\pi\xi)
    d\xi+\cancel{2f\int_0^1(\xi-1/2)\sin^2(2\pi\xi)d\xi}\\
    H_{2,2} &= 4\int_0^1\left[1-\cos(4\pi\xi)\right] \\
    H_{2,2} &= 4\left[\xi-\frac{1}{4\pi}\sin(4\pi\xi)\right]_0^1 \\
    H_{2,2} &= 4 \\
    H_{1,2} &= -\frac{1}{\pi^2} \int_0^1 \psi_i^*(\xi) \frac{d^2}{d\xi^2}
    \psi_j(\xi) d\xi + f\int_0^1 \psi_i^*(\xi)(\xi - 1/2)\psi_j(\xi) d\xi \\
    &
    \begin{aligned}
      \psi_i^*(\xi) &= \sqrt{2}\sin(\pi\xi) \\
      \psi_j(\xi) &= \sqrt{2}\sin(2\pi\xi) \\
      \frac{d^2}{d\xi^2} \psi_j(\xi) &=
      -4\sqrt{2}\pi^2\sin(2\pi\xi) \\
    \end{aligned}
  \end{align*}

}

\boxedanswer{
  \begin{align*}
    H_{1,2} &= -\frac{1}{\pi^2} \int_0^1 \left(\sqrt{2}\sin(\pi\xi)\right)
    \left(-4\sqrt{2}\pi^2\sin(2\pi\xi)\right)d\xi+
    f\int_0^1 \left(\sqrt{2}\sin(\pi\xi)\right)(\xi - 1/2)
    \left(\sqrt{2}\sin(2\pi\xi)\right) d\xi \\
    H_{1,2} &= 8\underbrace{\int_0^1 \overbrace{\sin(\pi\xi)}^{\text{even}}
    \overbrace{\sin(2\pi\xi)}^{\text{odd}}d\xi}_0 -
    2\overbrace{f}^3\overbrace{\int_0^1 (\xi - 1/2)\sin(\pi\xi)
    \sin(2\pi\xi)}^{\frac{8}{9\pi^2}}d\xi \\
    H_{1,2} &= -\frac{16}{3\pi^2} \\
    H_{2,1} &= -\frac{1}{\pi^2} \int_0^1 \psi_i^*(\xi) \frac{d^2}{d\xi^2}
    \psi_j(\xi) d\xi + f\int_0^1 \psi_i^*(\xi)(\xi - 1/2)\psi_j(\xi) d\xi \\
    &
    \begin{aligned}
      \psi_i^*(\xi) &= \sqrt{2}\sin(2\pi\xi) \\
      \psi_j(\xi) &= \sqrt{2}\sin(\pi\xi) \\
      \frac{d^2}{d\xi^2} \psi_j(\xi) &=
      -\sqrt{2}\pi^2\sin(2\pi\xi) \\
    \end{aligned} \\
    H_{2,1} &= -\frac{1}{\pi^2} \int_0^1
    \left(\sqrt{2}\sin(2\pi\xi)\right)\left(-\sqrt{2}\pi^2\sin(\pi\xi)\right)d\xi+
    f\int_0^1 \left(\sqrt{2}\sin(2\pi\xi)\right)(\xi - 1/2)
    \left(\sqrt{2}\sin(\pi\xi)\right) d\xi \\
    H_{2,1} &= \underbrace{\int_0^1 \overbrace{\sin(2\pi\xi)}^{\text{odd}}
    \overbrace{\sin(\pi\xi)}^{\text{even}}d\xi}_0 -
    2\overbrace{f}^3\overbrace{\int_0^1 (\xi - 1/2)\sin(\pi\xi)
    \sin(2\pi\xi)}^{\frac{8}{9\pi^2}}d\xi \\
    H_{2,1} &= -\frac{16}{3\pi^2} \\
    &\hat H =
    \begin{bmatrix}
      1 & -\frac{16}{3\pi^2} \\
      -\frac{16}{3\pi^2} & 4 \\
    \end{bmatrix} \\
    \hat H \phi(\xi) &= \eta \phi(\xi) \\
    \phi(\eta) &=c_1\psi_1(\xi) + c_2\psi_2(\xi) \\
    |\hat H- \eta I|c &= 0 \\
    & a = \frac{16}{3\pi^2} \\
    0 &=
    \begin{bmatrix}
      1 - \eta & -a \\
      -a & 4 - \eta \\
    \end{bmatrix}
    \begin{bmatrix}
      c_1 \\ c_2
    \end{bmatrix} \\
    0 &= (1 - \eta)c_1 - ac_2 \\
    0 &= -ac_1 + (4 - \eta)c_2 \\
    c_2 &= \frac{1 - \eta}{a}c_1 \\
    c &\propto
    \begin{bmatrix}
      1 \\ \frac{1 - \eta}{a} \\
    \end{bmatrix} \\
    c &= \frac{1}{\sqrt{1 + \left(\frac{1 - \eta}{a}\right)^2}}
    \begin{bmatrix}
      1 \\ \frac{1 - \eta}{a} \\
    \end{bmatrix} \\
    \left|\hat H - \eta I\right| &= (1 - \eta)(4 - \eta) - a^2 = 0 \\
    0 &= \underbrace{1}_d\eta^2 \underbrace{- 5}_b\eta +
    \underbrace{4 - a^2}_c \\
    \eta &= \frac{-b \pm \sqrt{b^2 - 4dc}}{2d}
  \end{align*}
}

\boxedanswer{
  \begin{align*}
    \eta &= \frac{-(5) \pm \sqrt{(-5)^2 - 4(1)(4-a^2)}}{2d} \\
    \eta &= \frac{5}{2} \pm \sqrt{\frac{9}{4} + a^2} \\
    \Aboxed{\eta &= \frac{5}{2} \pm \sqrt{\frac{9}{4} +
    \left(\frac{16}{3\pi^2}\right)^2}} \\
    c_1 &= \frac{1}{\sqrt{1 + \left(\frac{1 - \frac{5}{2} - \sqrt{\frac{9}{4} +
    \left(\frac{16}{3\pi^2}\right)^2}}{\frac{16}{3\pi^2}}\right)^2}}
    \begin{bmatrix}
      1 \\ \frac{1 - \frac{5}{2} - \sqrt{\frac{9}{4} +
      \left(\frac{16}{3\pi^2}\right)^2}}{\frac{16}{3\pi^2}} \\
    \end{bmatrix} \\
    c_1 &=
    \begin{bmatrix}\frac{16\sqrt{2}}{\sqrt{81\pi ^4+9\pi
      ^2\sqrt{81\pi ^4+1024}+1024}}\\ \frac{-9\pi ^2-\sqrt{81\pi
      ^4+1024}}{\sqrt{2}\sqrt{81\pi ^4+9\pi ^2\sqrt{81\pi ^4+1024}+1024}}\\ 0
    \end{bmatrix} \\
    c_2 &= \frac{1}{\sqrt{1 + \left(\frac{1 - \frac{5}{2} + \sqrt{\frac{9}{4} +
    \left(\frac{16}{3\pi^2}\right)^2}}{\frac{16}{3\pi^2}}\right)^2}}
    \begin{bmatrix}
      1 \\ \frac{1 - \frac{5}{2} + \sqrt{\frac{9}{4} +
      \left(\frac{16}{3\pi^2}\right)^2}}{\frac{16}{3\pi^2}} \\
    \end{bmatrix} \\
    c_2 &=
    \begin{bmatrix}\frac{16\sqrt{2}}{\sqrt{81\pi ^4-9\pi
      ^2\sqrt{81\pi ^4+1024}+1024}}\\ \frac{-9\pi ^2+\sqrt{81\pi
      ^4+1024}}{\sqrt{2}\sqrt{81\pi ^4-9\pi ^2\sqrt{81\pi ^4+1024}+1024}}\\
    \end{bmatrix} \\
    &\boxed{\phi_1 =
      \begin{bmatrix}\frac{16\sqrt{2}}{\sqrt{81\pi ^4+9\pi
        ^2\sqrt{81\pi ^4+1024}+1024}}\\ \frac{-9\pi ^2-\sqrt{81\pi
        ^4+1024}}{\sqrt{2}\sqrt{81\pi ^4+9\pi ^2\sqrt{81\pi ^4+1024}+1024}}\\
      \end{bmatrix}
      \begin{bmatrix}
        \sqrt{2}\sin(\pi\xi) & \sqrt{2}\sin(2\pi\xi) \\
    \end{bmatrix}} \\
    &\boxed{\phi_2 =
      \begin{bmatrix}\frac{16\sqrt{2}}{\sqrt{81\pi ^4-9\pi
        ^2\sqrt{81\pi ^4+1024}+1024}}\\ \frac{-9\pi ^2+\sqrt{81\pi
        ^4+1024}}{\sqrt{2}\sqrt{81\pi ^4-9\pi ^2\sqrt{81\pi ^4+1024}+1024}}\\
      \end{bmatrix}
      \begin{bmatrix}
        \sqrt{2}\sin(\pi\xi) & \sqrt{2}\sin(2\pi\xi) \\
    \end{bmatrix}}
  \end{align*}
}

\pagebreak% }}}

\section*{Problem 6.3.2}

Consider an electron in a one-dimensional potential well of width $L_z$,
with infinitely high barriers on either side, and in which the
potential energy
inside the potential well is parabolic, of the form

\begin{equation}
  V(z)=u(z-L_z/2)^2
\end{equation}

where $u$ is a real constant. This potential is presumed to be small
compared to the energy E1 of the first confined state of a simple rectangular
potential well of the same width $L_z$.
[Note for interest: This kind of situation can arise in semiconductor
  structures, where the parabolic curvature comes from the
electrostatic potential of uniform background doping of the material.]

Find an approximate expression, valid in the limit of small $u$, for
the transition energy between the first and second allowed states of this well
in terms of $u$, $L_z$, and fundamental constants.

\boxedanswer{
  We will use time-inependent perterbation theory to solve this problem:

  The unperturbed system is as follows:
  \begin{equation*}
    \hat H_0 | \psi_n \rangle = E_n | \psi_n\rangle \\
  \end{equation*}

  The perturbation Hamiltonian can be written:

  \begin{equation*}
    \hat H_p = u(z - L_z/2)^2 \\
  \end{equation*}

  The Schr\"odinger equation now becomes:

  \begin{equation*}
    (\hat H_o + \gamma \hat H_p) | \phi \rangle = E | \phi \rangle \\
  \end{equation*}

  We expand $|\phi\rangle$ in a power series of $\gamma$:

  \begin{align*}
    |\phi\rangle &= |\phi^{(0)}\rangle + \gamma |\phi^{(1)}\rangle +
    \gamma^2|\phi^{(2)}\rangle + \gamma^3|\phi^{(3)}\rangle+\cdots \\
    E &= E^{(0)} + \gamma E^{(1)} + \gamma^2E^{(2)} +\gamma^3E^{(3)} + \cdots
  \end{align*}

  Substituting:

  \begin{multline*}
    (\hat H_o + \gamma \hat H_p)\left(|\phi^{(0)}\rangle + \gamma
      |\phi^{(1)}\rangle +
    \gamma^2|\phi^{(2)}\rangle + \gamma^3|\phi^{(3)}\rangle+\cdots\right)  = \\
    \left(E^{(0)} + \gamma E^{(1)} + \gamma^2E^{(2)} +\gamma^3E^{(3)} + \cdots
    \right)\left(|\phi^{(0)}\rangle + \gamma |\phi^{(1)}\rangle +
    \gamma^2|\phi^{(2)}\rangle + \gamma^3|\phi^{(3)}\rangle+\cdots  \right) \\
  \end{multline*}

  Comparing terms that are in 0\textsuperscript{th} order in $\gamma$:

  \begin{align*}
    \hat H_0 | \phi^{(0)} \rangle &= E^{(0)} | \phi^{(0)} \rangle
  \end{align*}

  The is the unperturbed Hamiltonian, so $\phi^{(0)} = |\psi_m\rangle$.

  \begin{align*}
    \hat H_0 | \psi_m \rangle &= E_m | \psi_m \rangle
  \end{align*}

  Then the terms in 1\textsuperscript{st} and 2\textsuperscript{nd}
  order in $\gamma$:

  \begin{align*}
    \hat H_o | \phi^{(1)} \rangle + \hat H_p|\psi_m\rangle &=
    E_m | \phi^{(1)} \rangle + E^{(1)} \psi_m \rangle \\
    \hat H_o | \phi^{(2)}\rangle + \hat H_p|\phi^{(1)}\rangle &=
    E_m| \phi^{(2)} \rangle + E^{(1)} | \phi^{(1)}\rangle +
    E^{(2)}|\psi_m\rangle \\
  \end{align*}

}

\boxedanswer{

  Rearranging:

  \begin{align*}
    (\hat H_o - E_m) |\psi_m \rangle &= 0 \\
    (\hat H_o - E_m) | \phi^{(1)} \rangle &=
    (E^{(1)} - \hat H_p) |\phi^{(1)} \rangle \\
    (\hat H_o - E_m) |\phi^{(2)}\rangle &= (E^{(1)} - \hat H_p ) |
    \phi^{(1)} \rangle + E^{(2)} |\psi_m\rangle
  \end{align*}

  We then solve for the first-order correction eigenenergy:

  \begin{align*}
    \langle \psi_m |(\hat H_o - E_m) | \phi^{(1)} \rangle &=
    \langle \psi_m |(E^{(1)} - \hat H_p) |\phi^{(1)} \rangle \\
    \langle \psi_m | \hat H_o - E_m | \phi^{(1)} \rangle &=
    (\langle \psi_m | \hat H_o - E_m ) | \phi^{(1)} \rangle =
    \langle \psi_m | (E_m - E_m ) | \phi^{(1)} \rangle = 0 \\
    &= \langle \psi_m | E^{(1)} - \hat H_p | \psi_m\rangle
    = E^{(1)} - \langle \psi_m | \hat H_p | \psi_m\rangle \\
    E^{(1)} &= \langle \psi_m | \hat H_p | \psi_m\rangle
  \end{align*}

  Solve for the first-order correction by substituting into the first-order
  equation and multiply by a particular $\psi_i$:

  \begin{align*}
    | \phi^{(1)} \rangle &= \sum_n a_n^{(1)} | \psi_n \rangle \\
    \langle \psi_i | \hat H_o - E_m | \phi^{(1)} \rangle &= (E_i - E_m)
    \langle \psi_i | \phi^{(1)} \rangle = (E_i - E_m) a_i^{(1)} \\
    &= \langle \psi_i | E^{(1)} - \hat H_p | \psi_m \rangle = E^{(1)}
    \langle \psi_i | \psi_m \rangle - \langle \psi_i | \hat H_p |
    \psi_m \rangle \\
  \end{align*}

  Assuming non-degeneracy and $i \ne m$:

  \begin{align*}
    a_i^{(1)} &=  \frac{\langle \psi_i | \hat H_p |
    \psi_m \rangle}{E_m - E_i}
  \end{align*}

  For $i = m$:

  \begin{align*}
    (E_m - E_m)a_m^{(1)} &= 0 a_m^{(1)} \\
    &= E^{(1)} - \langle \psi_m | \hat H_p | \psi_m \rangle
    = E^{(1)} - E^{(1)} = 0
  \end{align*}

  For convenience, we can choose $a_m^{(1)} = 0$. Therefore:

  \begin{equation*}
    \langle \psi_m | \phi^{(j)} \rangle = 0
  \end{equation*}

  Hence:

  \begin{equation*}
    | \phi^{(1)} \rangle = \sum_{n \ne m} \frac{\langle \psi_n | \hat
    H_p | \psi_m \rangle}{E_m - E_n} | \psi_n \rangle
  \end{equation*}

  For this problem , we chose the basis functions to be the first two
  eigenfunctions for the infinite well.

  \begin{align*}
    \psi_m &= \sqrt{2}\sin\left(\frac{m\pi z}{L_z}\right) \\
    \Delta E_{1\rightarrow 2} &= E_2 - E_1 \\
    &
    \begin{aligned}
      E^{(1)} &= \langle \psi_m | \hat H_p | \psi_m \rangle \\
      E^{(1)} &= \int_0^{L_z} \sqrt{2} \sin\left(\frac{m\pi z}{L_z}\right)
      u(z - L_z/2)^2\sqrt{2}\sin\left(\frac{m\pi z}{L_z}\right)dz
    \end{aligned}
  \end{align*}

}

\boxedanswer{
  \begin{align*}
    E^{(1)} &= 2\int_0^{L_z}\sin\left(\frac{m\pi z}{L_z}\right)
    u(z - L_z/2)^2\sin\left(\frac{m\pi z}{L_z}\right)dz \\
    E^{(1)} &= 2u\int_0^{L_z}\sin^2\left(\frac{m\pi z}{L_z}\right)
    (z - L_z/2)^2dz \\
    E^{(1)} &= 2u\int_0^{L_z}\sin^2\left(\frac{m\pi z}{L_z}\right)
    (z^2 - zL_z + (L_z/2)^2)dz \\
    E^{(1)}_1 &= 2u\int_0^{L_z}z^2\sin^2\left(\frac{\pi z}{L_z}\right) dz
    - 2uL_z\int_0^{L_z}z\sin^2\left(\frac{\pi z}{L_z}\right) dz
    + \frac{2uL_z^2}{4}\int_0^{L_z}\sin^2\left(\frac{\pi z}{L_z}\right) dz \\
    &
    \begin{aligned}
      2u\int_0^{L_z}z^2\sin^2\left(\frac{\pi z}{L_z}\right) dz &=
      \frac{\left(2\pi^{2} - 3\right) L_{z}^{3} u}{6\pi^{2}} \\
      2uL_z\int_0^{L_z}z\sin^2\left(\frac{\pi z}{L_z}\right) dz &=
      \frac{L_{z}^{3} u}{2} \\
      \frac{2uL_z^2}{4}\int_0^{L_z}\sin^2\left(\frac{\pi z}{L_z}\right) dz &=
      \frac{L_{z}^{3} u}{4}
    \end{aligned} \\
    E^{(1)}_1 &= \frac{\left(2\pi^{2} - 3\right) L_{z}^{3} u}{6\pi^{2}}
    - \frac{L_{z}^{3} u}{2}
    + \frac{L_{z}^{3} u}{4} \\
    E^{(1)}_1 &= \frac{\left(\pi^{2} - 6\right) L_{z}^{3} u}{12\pi^{2}} \\
    E^{(1)}_2 &= 2u\int_0^{L_z}\sin^2\left(\frac{2\pi z}{L_z}\right)
    (z - L_z/2)^2dz \\
    E^{(1)}_2 &= 2u\int_0^{L_z}z^2\sin^2\left(\frac{2\pi z}{L_z}\right) dz
    - 2uL_z\int_0^{L_z}z\sin^2\left(\frac{2\pi z}{L_z}\right) dz
    + \frac{2uL_z^2}{4}\int_0^{L_z}\sin^2\left(\frac{2\pi z}{L_z}\right) dz \\
    &
    \begin{aligned}
      2u\int_0^{L_z}z^2\sin^2\left(\frac{2\pi z}{L_z}\right) dz &=
      \frac{\left(8\pi^{2} - 3\right) L_{z}^{3} u}{24\pi^{2}}\\
      2uL_z\int_0^{L_z}z\sin^2\left(\frac{2\pi z}{L_z}\right) dz &=
      \frac{L_{z}^{3} u}{2} \\
      \frac{2uL_z^2}{4}\int_0^{L_z}\sin^2\left(\frac{2\pi z}{L_z}\right) dz &=
      \frac{L_{z}^{3} u}{4}\\
    \end{aligned} \\
    E^{(1)}_2 &=\frac{\left(2\pi^{2} - 3\right) L_{z}^{3} u}{24\pi^{2}} \\
    \Aboxed{\Delta E^{(1)}_{1 \rightarrow 2} &= \frac{3L_{z}^{3} u}{8\pi^{2}}}
  \end{align*}
}

\pagebreak

\section*{Problem 7.1.2}

Consider a one-dimensional semiconductor potential well of width Lz with
potential barriers on either side approximated as being infinitely high. An
electron in this potential well is presumed to behave with an effective mass
$m_{eff}$. Initially, there is an electron in the lowest state of this
potential well. We want to use this semiconductor structure as a detector for
a very short electric field pulse. If the electron is found in the second
energy state after the pulse, the electron is presumed to be collected as
photocurrent by some mechanism, and the pulse is therefore detected.

To model this device, we presume that the electric field pulse F (t ) can be
approximated as a “half-cycle” pulse of length Δt , i.e., a pulse of the form

\begin{equation*}
  F(t) = F_0\sin\left(\frac{\pi t}{\Delta t} \right)
\end{equation*}

for times $t$ from $0$ to $\Delta t$, and zero for all other times.

\begin{enumerate}[(i)]
  \item Find an approximate expression, valid for sufficiently small field
    amplitude $F_o$, for the probability of finding the electron in its
    second state after the pulse.
  \item For a pulse of length $\Delta t = \SI{100}{\femto\second}$, and a
    \ch{GaAs} semiconductor structure with $m_{eff} = 0.07m_o$ and
    width $L_z = \SI{10}{\nano\meter}$, for what minimum electric field
    magnitude $F_o$ does this detector have at least a \SI{1}{\percent}
    chance of detecting the pulse?
  \item For a full cycle pulse (i.e., one of the form $F(t) =
      F_o\sin(2\pi t/\Delta t)$
      for times $t$ from $0$ to $\Delta t$, and zero for all other
    times), what is the probability of detecting the pulse with this detector?
    Justify your answer.
\end{enumerate}

\pagebreak

\end{document}
